Experiments.thy
@@ -38,7 +38,20 @@ ML \<open>val test = @{code test}\<close>
 ML \<open>test ()\<close>
 ML \<open>Timing.timeit test\<close>*)
 
+value "the (compute_ivl_bound_naive 32 10 [Ivl (-1) 1] (Cos (Var 0)))"
 value "the (compute_ivl_bound_naive 32 0 [Ivl (-1) 1] (Add (Power (Cos (Var 0)) 2) (Power (Sin (Var 0)) 2)))"
 value "the (compute_ivl_bound_naive 32 10 [Ivl (-1) 1] (Add (Power (Cos (Var 0)) 2) (Power (Sin (Var 0)) 2)))"
+
+value "the (compute_tm 32 10 [Ivl (-1) 1] [0] (Cos (Var 0)))"
+value "the (compute_tm 32 10 [Ivl (-1) 1] [0] (Cos (Add (Var 0) (Mult (Num 2) Pi))))"
+value "the (compute_tm 32 10 [Ivl (-1) 1] [0] (Add (Power (Cos (Var 0)) 2) (Power (Sin (Var 0)) 2)))"
+value "the (compute_tm 32 10 [Ivl (2) 6] [4] (Add (Power (Cos (Var 0)) 2) (Power (Sin (Var 0)) 2)))"
+
+value "the (compute_ivl_bound 32 10 [Ivl (-1) 1] (Cos (Var 0)))"
+value "the (compute_ivl_bound 32 10 [Ivl (-1) 1] (Cos (Add (Var 0) (Mult (Num 2) Pi))))"
+value "the (compute_ivl_bound 32 10 [Ivl (-1) 1] (Add (Power (Cos (Var 0)) 2) (Power (Sin (Var 0)) 2)))"
+value "the (compute_ivl_bound 32 10 [Ivl (1) 2] (Add (Power (Cos (Var 0)) 2) (Power (Sin (Var 0)) 2)))"
+
+find_theorems "_ (Float _ _) = (_ :: real)"
 
 end
